intermediate2/Zeta.Intermediate.StateRel.fsti
@@ -52,6 +52,16 @@ val lemma_runapp_simulates_spec
           (ensures (let ek = to_logk_entry vs e in
                     vtls_rel (GV.verify_step e vs) (GV.verify_step ek vs')))
 
+val lemma_app_res_rel
+  (#vcfg:_)
+  (vs: vtls_t vcfg{vs.valid})
+  (vs': _ {vtls_rel vs vs'})
+  (e: logS_entry vcfg {GV.is_appfn e})
+  : Lemma (requires (valid_logS_entry vs e /\ (GV.verify_step e vs).valid))
+          (ensures (let ek = to_logk_entry vs e in
+                    vtls_rel (GV.verify_step e vs) (GV.verify_step ek vs') /\
+                    GV.appfn_result e vs = GV.appfn_result ek vs'))
+
 (* adding a key not in store to vaddm preserves the spec relationship *)
 val lemma_vaddm_preserves_spec_new_key
       (#vcfg:_)
